#+title: Lösungen zum 6. Übungsblatt
#+date: 2018-05-30
#+email: tobias.denkinger@tu-dresden.de
#+options: toc:nil

* Lösung zu Aufgabe 1 (AGS 12.4.32)
** Teilaufgabe a
#+begin_src elisp
(λfx.ffx)(λy.x)z
   ----- ------
  GV={x} FV={x}

⇒ₐ (λfx₁.ffx₁)(λy.x)z

⇒ᵦ (λx₁.(λy.x)(λy.x)x₁)z
           -- -----
        GV=∅  FV={x}

⇒ᵦ (λx₁.xx₁)z
       --- --
     GV=∅  FV={z}

⇒ᵦ xz
#+end_src

** Teilaufgabe b
#+begin_src elisp
⟨Y⟩⟨F⟩
= (λh.(λy.h(yy))(λy.h(yy))) ⟨F⟩
⇒* (λy.⟨F⟩(yy))(λy.⟨F⟩(yy)) = ⟨Y_F⟩
⇒* ⟨F⟩ ((λy.⟨F⟩(yy))(λy.⟨F⟩(yy))) = ⟨F⟩ ⟨Y_F⟩

⟨Y⟩⟨F⟩⟨6⟩⟨5⟩⟨3⟩
⇒* ⟨F⟩ ⟨Y_F⟩ ⟨6⟩ ⟨5⟩ ⟨3⟩
⇒* ⟨ite⟩ (⟨iszero⟩(⟨sub⟩⟨6⟩⟨5⟩))
         (⟨add⟩⟨5⟩⟨3⟩)
         (⟨succ⟩ (⟨Y_F⟩ (⟨pred⟩⟨6⟩) (⟨succ⟩⟨5⟩) (⟨mult⟩⟨2⟩⟨3⟩)))
⇒* ⟨ite⟩ ⟨false⟩ (…) (⟨succ⟩ (⟨Y_F⟩ ⟨5⟩ ⟨6⟩ ⟨6⟩))
⇒* ⟨succ⟩ (⟨Y_F⟩ ⟨5⟩ ⟨6⟩ ⟨6⟩)
⇒* ⟨succ⟩ (⟨F⟩ ⟨Y_F⟩ ⟨5⟩ ⟨6⟩ ⟨6⟩)
⇒* ⟨succ⟩ (⟨ite⟩ (⟨iszero⟩(⟨sub⟩⟨5⟩⟨6⟩))
                 (⟨add⟩⟨6⟩⟨6⟩)
                 (⟨succ⟩ (⟨Y_F⟩(⟨pred⟩⟨5⟩)(⟨succ⟩⟨6⟩)(⟨mult⟩⟨2⟩⟨6⟩)))
          )
⇒* ⟨succ⟩ (⟨ite⟩ ⟨true⟩ ⟨12⟩ (…))
⇒* ⟨13⟩
#+end_src

** Teilaufgabe c
#+begin_src elisp
⟨G⟩ = (λgxy. ⟨ite⟩ (⟨iszero⟩x)
                   (⟨mult⟩ ⟨2⟩ (⟨succ⟩y))
                   (⟨ite⟩ (⟨iszero⟩y)
                          (⟨mult⟩ ⟨2⟩ (⟨succ⟩x))
                          (⟨add⟩ ⟨4⟩ (g (⟨pred⟩x) (⟨pred⟩y)))
                   )
      )
#+end_src

* Lösung zu Aufgabe 2 (AGS 13.1)
  **siehe sol06-2.pl**

* Lösung zu Aufgabe 3 (AGS 13.2)
#+begin_src prolog
            ?- prod(s(s(0)), s(0), X).
            ?- prod(s(0), s(0), W)                , sum(s(0), W, X).
            ?- prod(0, s(0), W1), sum(s(0), W1, W), sum(s(0), W, X).
{W1 = 0}    ?- prod(0, s(0), 0 ), sum(s(0), 0 , W), sum(s(0), W, X).
            ?- sum(s(0), 0 , W), sum(s(0), W, X).
{W = s(Z)}  ?- sum(s(0), 0, s(Z)), sum(s(0), s(Z), X).
            ?- sum(0, 0, Z), sum(s(0), s(Z), X).
{Z = 0}     ?- sum(0, 0, 0), sum(s(0), s(0), X).
            ?- sum(s(0), s(0), X).
{X = s(Z1)} ?- sum(s(0), s(0), s(Z1)).
            ?- sum(0, s(0), Z1).
{Z1 = s(0)} ?- sum(0, s(0), s(0)).
            ?-.

X = s(Z1) = s(s(0))
#+end_src
